Reorganize code

KeyManagement/RealWorld.v
@@ -1,51 +1,13 @@
 From Coq Require Import String Sumbool Morphisms.
 
-Require Import MyPrelude Common Maps.
+Require Import
+        MyPrelude
+        Common
+        Maps
+        Tactics
+        Keys.
 
 Set Implicit Arguments.
-
-Definition key_identifier := nat.
-
-Inductive key_usage :=
-| Encryption
-| Signing.
-
-Lemma key_usage_eq_dec :
-  forall u1 u2 : key_usage, { u1 = u2 } + { u1 <> u2 }.
-  decide equality.
-Defined.
-
-Inductive key_type :=
-| SymKey
-| AsymKey.
-
-Lemma key_type_eq_dec :
-  forall kt1 kt2 : key_type, { kt1 = kt2 } + { kt1 <> kt2 }.
-  decide equality.
-Defined.
-
-Record key :=
-  MkCryptoKey { keyId    : key_identifier
-              ; keyUsage : key_usage
-              ; keyType  : key_type
-              }.
-
-Lemma key_eq_dec :
-  forall k1 k2 : key, { k1 = k2 } + { k1 <> k2 }.
-  decide equality; auto using Nat.eq_dec, key_usage_eq_dec, key_type_eq_dec.
-Defined.
-
-Definition key_permission : Set := key_identifier * bool.
-
-Lemma key_permission_eq_dec :
-  forall kp1 kp2 : key_permission, { kp1 = kp2 } + { kp1 <> kp2 }.
-  decide equality; auto using Nat.eq_dec, Bool.bool_dec.
-Defined.
-
-Notation "x ==kk y" := (key_eq_dec x y) (right associativity, at level 75).
-Notation "x ==ku y" := (key_usage_eq_dec x y) (right associativity, at level 75).
-Notation "x ==kt y" := (key_type_eq_dec x y) (right associativity, at level 75).
-Notation "x ==kp y" := (key_permission_eq_dec x y) (right associativity, at level 75).
 
 Definition cipher_id := nat.
 
@@ -96,8 +58,6 @@ Definition cipher_signing_key (c : cipher) :=
   end.
 
 Definition queued_messages := list (sigT message).
-Definition keys            := NatMap.t key.
-Definition key_perms       := NatMap.t bool.
 Definition ciphers         := NatMap.t cipher.
 Definition my_ciphers      := list cipher_id.
 
@@ -112,16 +72,6 @@ Inductive msg_accepted_by_pattern : forall {t : type}, msg_pat -> message t -> P
     msg_accepted_by_pattern (Signed k) (Signature m k c_id)
 | ProperlyEncrypted : forall {t} c_id k__sign k__enc (m : message t),
     msg_accepted_by_pattern (SignedEncrypted k__sign k__enc) (SignedCiphertext k__sign k__enc c_id).
-
-Ltac context_map_rewrites :=
-  repeat
-    match goal with
-    | [ H : ?m $? ?k = _ |- context[?m $? ?k] ] => rewrite H
-    | [ H : match ?matchee with _ => _ end $? _ = _
-     ,  H1 : ?matchee = _ |- _] => rewrite H1 in H
-    | [ H : match ?matchee with _ => _ end = _
-     ,  H1 : ?matchee = _ |- _] => rewrite H1 in H
-    end.
 
 Hint Extern 1 (~ In _ _) => rewrite not_find_in_iff.
 
@@ -294,72 +244,6 @@ Record universe (A B : Type) :=
     ; all_keys    : keys
     }.
 
-Definition greatest_permission (kp1 kp2 : bool) : bool :=
-  kp1 || kp2.
-
-Definition add_key_perm (k : key_identifier)(kp : bool) (perms : key_perms) : key_perms :=
-    match perms $? k with
-    | None     => perms $+ (k, kp)
-    | Some kp' => perms $+ (k, greatest_permission kp kp')
-    end.
-
-Lemma greatest_permission_refl :
-  forall k,
-    greatest_permission k k = k.
-Proof.
-  unfold greatest_permission; auto using orb_diag.
-Qed.
-
-Lemma greatest_permission_symm :
-  forall kp1 kp2,
-    greatest_permission kp1 kp2 = greatest_permission kp2 kp1.
-Proof.
-  unfold greatest_permission; auto using orb_comm.
-Qed.
-
-Definition merge_perms (ks ks' : key_perms) : key_perms :=
-  fold add_key_perm ks ks'.
-
-Notation "m1 $k++ m2" := (merge_perms m2 m1) (at level 50, left associativity).
-
-Lemma add_key_perm_proper :
-  Proper (eq  ==>  eq  ==>  eq  ==>  eq ) add_key_perm.
-Proof.
-  unfold Proper, respectful; intros; subst; trivial.
-Qed.
-
-Lemma add_key_perm_proper_Equal :
-  Proper (eq  ==>  eq  ==>  Equal  ==>  Equal ) add_key_perm.
-Proof.
-  unfold Proper, respectful; intros; Equal_eq;
-    unfold Equal; intros; trivial.
-Qed.
-
-Lemma add_key_perm_transpose :
-  transpose_neqkey eq add_key_perm.
-Proof.
-  unfold transpose_neqkey, add_key_perm; intros.
-  apply map_eq_Equal; unfold Equal; intros;
-    cases (a $? k); cases (a $? k');
-      repeat (context_map_rewrites; clean_map_lookups);
-      cases (y ==n k); cases (y ==n k'); subst; clean_map_lookups; trivial; contradiction.
-Qed.
-
-Lemma add_key_perm_transpose_Equal :
-  transpose_neqkey Equal add_key_perm.
-Proof.
-  unfold transpose_neqkey, add_key_perm; intros.
-  unfold Equal; intros;
-    cases (a $? k); cases (a $? k');
-      repeat (context_map_rewrites; clean_map_lookups);
-      cases (y ==n k); cases (y ==n k'); subst; clean_map_lookups; trivial; contradiction.
-Qed.
-
-Hint Resolve
-     add_key_perm_proper       add_key_perm_transpose
-     add_key_perm_proper_Equal add_key_perm_transpose_Equal.
-
-
 Definition findUserKeys {A} (us : user_list (user_data A)) : key_perms :=
   fold (fun u_id u ks => ks $k++ u.(key_heap)) us $0.
 
@@ -371,7 +255,6 @@ Definition addUserKeys {A} (ks : key_perms) (u : user_data A) : user_data A :=
 
 Definition addUsersKeys {A} (us : user_list (user_data A)) (ks : key_perms) : user_list (user_data A) :=
   map (addUserKeys ks) us.
-
 
 Lemma Forall_app_sym :
   forall {A} (P : A -> Prop) (l1 l2 : list A),
@@ -400,12 +283,6 @@ Proof.
       eapply H;
       apply in_inv in H0; split_ors; subst; simpl; eauto.
 Qed.
-
-(* Definition message_queue_ok (msgs : queued_messages) (honestk : key_perms) := *)
-(*   Forall (fun sigm => match sigm with *)
-(*                    | (existT _ _ m) => *)
-(*                      msg_honestly_signed honestk m = true -> msg_contains_only_honest_public_keys honestk m *)
-(*                    end) msgs. *)
 
 Fixpoint findKeys {t} (msg : message t) : key_perms :=
   match msg with
@@ -452,342 +329,7 @@ Definition user_cipher_queue {A} (usrs : honest_users A) (u_id : user_id) : opti
   | None     => None
   end.
 
-Section KeyMergeTheorems.
-  Variable all_keys : keys.
-  Variable honestk advk : key_perms.
-
-  Hint Resolve empty_Empty.
-
-  Ltac progress_fold_add1 :=
-    match goal with
-    | [ H : fold add_key_perm (_ $+ (_,_)) _ $? _ = _ |- _ ] => rewrite fold_add in H
-    | [ H : _ $k++ (_ $+ (_,_)) $? _ = _ |- _ ] => unfold merge_perms in H; rewrite fold_add in H
-    | [ |- context[ fold add_key_perm (_ $+ (_,_)) _ ] ] => rewrite fold_add
-    | [ |- context[ _ $k++ (_ $+ (_,_))] ] => unfold merge_perms; rewrite fold_add
-    end.
-
-  Lemma merge_perms_notation :
-    forall ks1 ks2,
-      fold add_key_perm ks2 ks1 = ks1 $k++ ks2.
-    unfold merge_perms; trivial.
-  Qed.
-
-  Lemma merge_perms_left_identity :
-    forall ks,
-      $0 $k++ ks = ks.
-  Proof.
-    induction ks using P.map_induction_bis; intros; Equal_eq; auto.
-
-    progress_fold_add1; auto.
-    rewrite merge_perms_notation.
-    unfold add_key_perm; auto.
-    rewrite IHks; auto.
-    case_eq (ks $? x); intros; subst; clean_map_lookups; trivial.
-  Qed.
-
-  Lemma merge_keys_right_identity :
-    forall ks,
-      ks $k++ $0 = ks.
-  Proof.
-    unfold merge_perms; intros; rewrite fold_Empty; eauto.
-  Qed.
-
-  Hint Rewrite merge_keys_right_identity merge_perms_left_identity.
-
-  Lemma merge_perms_adds_no_new_perms :
-    forall ks2 k ks1,
-        ks1 $? k = None
-      -> ks2 $? k = None
-      -> (ks1 $k++ ks2) $? k = None.
-  Proof.
-    induction ks2 using P.map_induction_bis; intros; Equal_eq; auto.
-    progress_fold_add1; auto.
-    rewrite merge_perms_notation.
-    unfold add_key_perm.
-    case (x ==n k); intros; subst; clean_map_lookups.
-    cases (ks1 $k++ ks2 $? x); clean_map_lookups; auto.
-  Qed.
-
-  Hint Resolve merge_perms_adds_no_new_perms.
-
-  Lemma merge_perms_came_from_somewhere1 :
-    forall ks2 ks1 k v,
-        ks1 $k++ ks2 $? k = Some v
-      -> ks2 $? k = None
-      -> ks1 $? k = Some v.
-  Proof.
-    induction ks2 using P.map_induction_bis; intros; Equal_eq; auto.
-    case (x ==n k); intros; subst; clean_map_lookups.
-    progress_fold_add1; auto.
-    rewrite merge_perms_notation in *.
-    unfold add_key_perm in *.
-    cases (ks1 $k++ ks2 $? x); clean_map_lookups; auto.
-  Qed.
-
-  Lemma merge_perms_came_from_somewhere2 :
-    forall ks2 ks1 k v,
-        ks1 $k++ ks2 $? k = Some v
-      -> ks1 $? k = None
-      -> ks2 $? k = Some v.
-  Proof.
-    induction ks2 using P.map_induction_bis; intros; Equal_eq; eauto.
-    - rewrite merge_keys_right_identity in H; clean_map_lookups.
-    - case (k ==n x); intros; subst; clean_map_lookups;
-        progress_fold_add1; auto;
-          rewrite merge_perms_notation in *;
-          unfold add_key_perm in *.
-      + assert (ks1 $k++ ks2 $? x = None) by eauto.
-      context_map_rewrites; clean_map_lookups; auto.
-      + cases (ks1 $k++ ks2 $? x); clean_map_lookups; eauto.
-  Qed.
-
-  Hint Resolve merge_perms_came_from_somewhere1 merge_perms_came_from_somewhere2.
-
-  Lemma merge_perms_adds_ks1 :
-    forall ks2 ks1 k v ks,
-        ks1 $? k = Some v
-      -> ks2 $? k = None
-      -> ks = ks1 $k++ ks2
-      -> ks $? k = Some v.
-  Proof.
-    unfold merge_perms.
-    induction ks2 using P.map_induction_bis; intros; Equal_eq; eauto.
-    - subst; rewrite fold_Empty; eauto.
-    - case (x ==n k); intros; subst; clean_map_lookups; eauto.
-      progress_fold_add1; auto.
-      rewrite merge_perms_notation.
-      unfold add_key_perm.
-      cases ( ks1 $k++ ks2 $? x ); clean_map_lookups; eauto.
-  Qed.
-
-  Lemma merge_perms_adds_ks2 :
-    forall ks2 ks1 k v ks,
-        ks1 $? k = None
-      -> ks2 $? k = Some v
-      -> ks = ks1 $k++ ks2
-      -> ks $? k = Some v.
-  Proof.
-    unfold merge_perms.
-    induction ks2 using P.map_induction_bis; intros; Equal_eq; contra_map_lookup; eauto.
-    subst; progress_fold_add1; auto.
-    rewrite merge_perms_notation.
-    unfold add_key_perm.
-    cases (k ==n x); subst; clean_map_lookups.
-    + assert (ks1 $k++ ks2 $? x = None) by eauto.
-      context_map_rewrites; clean_map_lookups; auto.
-    + cases ( ks1 $k++ ks2 $? x); clean_map_lookups; eauto.
-  Qed.
-
-  Hint Resolve merge_perms_adds_ks1 merge_perms_adds_ks2.
-
-  Lemma merge_perms_chooses_greatest :
-    forall ks2 ks1 k k' kp kp',
-        ks1 $? k = Some kp
-      -> ks2 $? k' = Some kp'
-      -> k = k'
-      -> (ks1 $k++ ks2) $? k = Some (greatest_permission kp kp').
-  Proof.
-    induction ks2 using P.map_induction_bis; intros; Equal_eq; contra_map_lookup; eauto.
-    progress_fold_add1; auto.
-    rewrite merge_perms_notation.
-    unfold add_key_perm.
-    subst.
-    cases (x ==n k'); subst; clean_map_lookups.
-    + assert (ks1 $k++ ks2 $? k' = Some kp) by eauto.
-      context_map_rewrites; clean_map_lookups; auto.
-      rewrite greatest_permission_symm; trivial.
-    + cases (ks1 $k++ ks2 $? x); subst; clean_map_lookups; eauto.
-  Qed.
-
-  Hint Resolve merge_perms_chooses_greatest.
-
-  Lemma merge_perms_split :
-    forall ks2 ks1 k kp,
-      ks1 $k++ ks2 $? k = Some kp
-      -> ks1 $? k = Some kp
-      \/ ks2 $? k = Some kp.
-  Proof.
-    induction ks2 using P.map_induction_bis; intros; Equal_eq; auto.
-    cases (x ==n k); subst; clean_map_lookups; auto;
-      progress_fold_add1; auto;
-        rewrite merge_perms_notation in *;
-        unfold add_key_perm in *.
-
-    + subst. clean_map_lookups.
-      cases (ks1 $k++ ks2 $? k); clean_map_lookups; auto.
-      apply merge_perms_came_from_somewhere1 in Heq; auto.
-      unfold greatest_permission; cases e; cases b; simpl; auto.
-
-    + cases (ks1 $k++ ks2 $? x); clean_map_lookups; auto.
-  Qed.
-
-  Lemma merge_perms_no_disappear_perms :
-    forall ks2 k ks1,
-      ks1 $k++ ks2 $? k = None
-    -> ks1 $? k = None
-    /\ ks2 $? k = None.
-  Proof.
-    induction ks2 using P.map_induction_bis; intros; Equal_eq; auto.
-    progress_fold_add1; auto.
-    rewrite merge_perms_notation in *; clean_map_lookups.
-    unfold add_key_perm in *.
-    cases (ks1 $k++ ks2 $? x);
-      cases (x ==n k); subst; clean_map_lookups; auto.
-  Qed.
-
-  Lemma merge_keys_neq_add_ok :
-    forall ks2 ks1 k k' kp,
-      k <> k'
-      -> ks1 $+ (k,kp) $k++ ks2 $? k' = ks1 $k++ ks2 $? k'.
-  Proof.
-    intros.
-    cases (ks1 $? k'); cases (ks2 $? k').
-    - erewrite !merge_perms_chooses_greatest; clean_map_lookups; eauto.
-    - erewrite !merge_perms_adds_ks1; auto; clean_map_lookups; eauto.
-    - erewrite !merge_perms_adds_ks2; auto; clean_map_lookups; eauto.
-    - erewrite !merge_perms_adds_no_new_perms; clean_map_lookups; auto.
-  Qed.
-
-  Hint Resolve merge_keys_neq_add_ok.
-
-  Lemma merge_keys_pull1 :
-    forall ks2 ks1 k kp kp' gkp,
-        ks2 $? k = Some kp'
-      -> gkp = greatest_permission kp kp'
-      -> (ks1 $+ (k, kp)) $k++ ks2 = ks1 $k++ ks2 $+ (k, gkp).
-  Proof.
-    induction ks2 using P.map_induction_bis; intros; Equal_eq; contra_map_lookup; eauto.
-    apply map_eq_Equal; unfold Equal; intros.
-    cases (k ==n x); cases (k ==n y); cases (x ==n y); subst; clean_map_lookups; try contradiction.
-    - eapply merge_perms_chooses_greatest; auto; clean_map_lookups; trivial.
-    - unfold merge_perms at 1; rewrite fold_add; auto; rewrite merge_perms_notation; unfold add_key_perm.
-      assert (ks1 $+ (x, kp) $k++ ks2 $? x = Some kp) by (eapply merge_perms_adds_ks1; eauto; clean_map_lookups; trivial).
-      context_map_rewrites; clean_map_lookups.
-      unfold merge_perms at 2; rewrite fold_add; auto; rewrite merge_perms_notation with (ks1:=ks1); unfold add_key_perm.
-      cases (ks1 $k++ ks2 $? x); subst; clean_map_lookups; eauto.
-    - progress_fold_add1; auto.
-      rewrite merge_perms_notation; unfold add_key_perm.
-      cases (ks1 $+ (y, kp) $k++ ks2 $? x); clean_map_lookups; auto;
-        erewrite merge_perms_chooses_greatest; auto; clean_map_lookups; eauto.
-    - unfold merge_perms; rewrite !fold_add; auto.
-      rewrite merge_perms_notation. rewrite merge_perms_notation with (ks1:=ks1).
-      unfold add_key_perm.
-      cases (ks1 $k++ ks2 $? y); eauto.
-      + assert (ks1 $? y = Some b) by eauto.
-        assert (ks1 $+ (k, kp) $k++ ks2 $? y = Some b). eapply merge_perms_adds_ks1; auto. clean_map_lookups; auto. auto.
-        context_map_rewrites; clean_map_lookups; trivial.
-      + eapply merge_perms_no_disappear_perms in Heq; auto; split_ands.
-        assert (ks1 $+ (k, kp) $k++ ks2 $? y = None) by (apply merge_perms_adds_no_new_perms; clean_map_lookups; auto).
-        context_map_rewrites; clean_map_lookups; auto.
-    - unfold merge_perms; rewrite !fold_add; auto.
-      rewrite merge_perms_notation. rewrite merge_perms_notation with (ks1:=ks1).
-      unfold add_key_perm.
-      cases (ks1 $k++ ks2 $? x); clean_map_lookups.
-      + apply merge_perms_came_from_somewhere1 in Heq; eauto.
-        assert (ks1 $+ (k, kp) $k++ ks2 $? x = Some b). eapply merge_perms_adds_ks1; auto. clean_map_lookups; auto. auto.
-        context_map_rewrites; clean_map_lookups; auto.
-      + eapply merge_perms_no_disappear_perms in Heq; auto; split_ands.
-        assert (ks1 $+ (k, kp) $k++ ks2 $? x = None) by (apply merge_perms_adds_no_new_perms; clean_map_lookups; auto).
-        context_map_rewrites; clean_map_lookups; auto.
-  Qed.
-
-  Lemma merge_keys_pull2 :
-    forall ks2 ks1 k kp gkp,
-        ks2 $? k = None
-      -> gkp = kp
-      -> (ks1 $+ (k, kp)) $k++ ks2 = ks1 $k++ ks2 $+ (k, gkp).
-  Proof.
-    induction ks2 using P.map_induction_bis; intros; Equal_eq; autorewrite with core; subst; auto.
-    cases (x ==n k); subst; clean_map_lookups.
-    unfold merge_perms; rewrite !fold_add; auto.
-    rewrite merge_perms_notation. rewrite merge_perms_notation with (ks1:=ks1).
-    unfold add_key_perm.
-    cases (ks1 $k++ ks2 $? x).
-    - apply merge_perms_came_from_somewhere1 in Heq; auto.
-      assert (ks1 $+ (k, kp) $k++ ks2 $? x = Some b) by (eapply merge_perms_adds_ks1; trivial; clean_map_lookups; auto).
-      context_map_rewrites; clean_map_lookups; auto.
-      erewrite IHks2; auto.
-      apply map_eq_Equal; unfold Equal; intros.
-      cases (y ==n x); cases (y ==n k); subst; clean_map_lookups; auto; contradiction.
-    - apply merge_perms_no_disappear_perms in Heq; auto; split_ands.
-      assert (ks1 $+ (k, kp) $k++ ks2 $? x = None) by (apply merge_perms_adds_no_new_perms; clean_map_lookups; auto).
-      context_map_rewrites.
-      apply map_eq_Equal; unfold Equal; intros.
-      erewrite IHks2; auto.
-      cases (y ==n x); cases (y ==n k); subst; clean_map_lookups; auto; contradiction.
-  Qed.
-
-  Lemma merge_perms_sym :
-    forall ks2 ks1,
-      ks1 $k++ ks2 = ks2 $k++ ks1.
-  Proof.
-    induction ks2 using P.map_induction_bis; intros; Equal_eq; eauto.
-    - rewrite merge_keys_right_identity, merge_perms_left_identity; trivial.
-    - unfold merge_perms at 1; rewrite fold_add; auto.
-      rewrite merge_perms_notation.
-      unfold add_key_perm; simpl.
-
-      cases (ks1 $k++ ks2 $? x); subst; clean_map_lookups.
-      + apply merge_perms_came_from_somewhere1 in Heq; auto.
-        erewrite merge_keys_pull1; eauto; rewrite IHks2; auto.
-      + apply merge_perms_no_disappear_perms in Heq; auto; split_ands.
-        erewrite merge_keys_pull2; eauto; rewrite IHks2; auto.
-  Qed.
-
-  Lemma merge_perms_refl :
-    forall ks,
-      ks $k++ ks = ks.
-  Proof.
-    induction ks using P.map_induction_bis; intros; Equal_eq; auto.
-    progress_fold_add1; auto.
-    rewrite merge_perms_notation.
-    unfold add_key_perm.
-    erewrite merge_keys_pull2; clean_map_lookups; auto.
-    rewrite map_add_eq, IHks; rewrite greatest_permission_refl; trivial.
-  Qed.
-
-  Lemma merge_perms_assoc :
-    forall ks3 ks1 ks2,
-      ks1 $k++ ks2 $k++ ks3 = ks1 $k++ (ks2 $k++ ks3).
-  Proof.
-    induction ks3 using P.map_induction_bis; intros; Equal_eq; auto.
-    unfold merge_perms at 1.
-    unfold merge_perms at 3.
-    rewrite !fold_add; auto.
-    rewrite merge_perms_notation.
-    rewrite merge_perms_notation with (ks1:=ks2).
-    unfold add_key_perm.
-
-    cases (ks2 $k++ ks3 $? x).
-    - cases (ks1 $k++ ks2 $k++ ks3 $? x);
-        subst; rewrite IHks3 in Heq0; clean_map_lookups; eauto.
-      + cases (ks1 $? x).
-        * assert (ks1 $k++ (ks2 $k++ ks3) $? x = Some (greatest_permission b1 b)) by eauto.
-          clean_map_lookups.
-          apply map_eq_Equal; unfold Equal; intros.
-          cases (y ==n x); subst; clean_map_lookups.
-          ** assert (ks1 $k++ (ks2 $k++ ks3 $+ (x, greatest_permission e b)) $? x = Some (greatest_permission b1 (greatest_permission e b)))
-              by (eapply merge_perms_chooses_greatest; auto; clean_map_lookups; auto).
-             context_map_rewrites; unfold greatest_permission.
-             rewrite !orb_assoc, orb_comm with (b1:=e); trivial.
-          ** symmetry; rewrite merge_perms_sym.
-             rewrite merge_keys_neq_add_ok, merge_perms_sym, <- IHks3; auto; trivial.
-        * assert (ks1 $k++ (ks2 $k++ ks3) $? x = Some b) by eauto; clean_map_lookups.
-          apply map_eq_Equal; unfold Equal; intros.
-          cases (y ==n x); subst; clean_map_lookups.
-          ** assert (ks1 $k++ (ks2 $k++ ks3 $+ (x, greatest_permission e b)) $? x = Some (greatest_permission e b))
-              by (eapply merge_perms_adds_ks2; auto; clean_map_lookups; auto).
-             context_map_rewrites; eauto.
-          ** symmetry; rewrite merge_perms_sym.
-             rewrite merge_keys_neq_add_ok, merge_perms_sym, <- IHks3; auto; trivial.
-
-      + apply merge_perms_no_disappear_perms in Heq0; auto; split_ands; contra_map_lookup.
-
-    - unfold merge_perms at 7.
-      rewrite fold_add; auto.
-      unfold add_key_perm at 1. rewrite merge_perms_notation with (ks2:=ks2 $k++ ks3).
-      rewrite IHks3; trivial.
-  Qed.
+Section RealWorldLemmas.
 
   Lemma findUserKeys_foldfn_proper :
     forall {A},
@@ -943,11 +485,11 @@ Section KeyMergeTheorems.
       rewrite findUserKeys_notation.
       cases (findUserKeys usrs $? k); subst.
       + erewrite merge_perms_chooses_greatest; eauto; unfold greatest_permission; rewrite orb_true_r; auto.
-      + erewrite merge_perms_came_from_somewhere2; eauto.
+      + erewrite merge_perms_adds_ks2; eauto.
     - unfold findUserKeys; rewrite fold_add; auto; rewrite findUserKeys_notation; eauto.
       cases (key_heap e $? k); subst; auto.
       + erewrite merge_perms_chooses_greatest; eauto; unfold greatest_permission; rewrite orb_true_l; auto.
-      + erewrite merge_perms_came_from_somewhere1; eauto.
+      + erewrite merge_perms_adds_ks1 with (ks1:=findUserKeys usrs); eauto.
   Qed.
 
   Lemma findUserKeys_readd_user_same_key_heap_idempotent :
@@ -975,19 +517,20 @@ Section KeyMergeTheorems.
   Qed.
 
   Lemma honest_key_after_new_keys :
-    forall msgk k_id,
+    forall honestk msgk k_id,
         honest_key honestk k_id
       -> honest_key (honestk $k++ msgk) k_id.
   Proof.
     invert 1; intros; econstructor; eauto.
     cases (msgk $? k_id); subst; eauto.
-    erewrite merge_perms_chooses_greatest by eauto; eauto.
+    - erewrite merge_perms_chooses_greatest by eauto; eauto.
+    - erewrite merge_perms_adds_ks1; eauto.
   Qed.
 
   Hint Resolve honest_key_after_new_keys.
 
   Lemma honest_keyb_after_new_keys :
-    forall msgk k_id,
+    forall honestk msgk k_id,
       honest_keyb honestk k_id = true
       -> honest_keyb (honestk $k++ msgk) k_id = true.
   Proof.
@@ -997,7 +540,7 @@ Section KeyMergeTheorems.
   Hint Resolve honest_keyb_after_new_keys.
 
   Lemma not_honest_key_after_new_msg_keys :
-    forall {t} (msg : message t) k,
+    forall {t} (msg : message t) honestk k,
       ~ honest_key honestk k
       -> (forall (k_id : NatMap.key) (kp : bool), findKeys msg $? k_id = Some kp -> kp = false)
       -> ~ honest_key (honestk $k++ findKeys msg) k.
@@ -1008,24 +551,19 @@ Section KeyMergeTheorems.
       erewrite merge_perms_chooses_greatest in H2; unfold greatest_permission in *; eauto.
       rewrite orb_false_l in H2; invert H2.
       specialize (H0 _ _ Heq0); discriminate.
+    - cases b; eauto.
+      erewrite merge_perms_adds_ks1 in H2; eauto.
+      discriminate.
     - erewrite merge_perms_adds_ks2 in H2; eauto.
       invert H2.
       specialize (H0 _ _ Heq0); discriminate.
+    - rewrite merge_perms_adds_no_new_perms in H2; eauto; discriminate.
   Qed.
 
   Hint Resolve not_honest_key_after_new_msg_keys.
 
-  (* Lemma message_honestly_signed_after_new_msg_keys : *)
-  (*   forall {t} (msg : message t) msgk, *)
-  (*     msg_honestly_signed honestk msg = true *)
-  (*     -> msg_honestly_signed (honestk $k++ msgk) msg = true. *)
-  (* Proof. *)
-  (*   induction msg; intros; simpl in *; eauto. *)
-  (*   rewrite andb_true_iff in *; split_ands; auto. *)
-  (* Qed. *)
-
   Lemma message_honestly_signed_after_add_keys :
-    forall {t} (msg : message t) ks,
+    forall {t} (msg : message t) honestk ks,
       msg_honestly_signed honestk msg = true
       -> msg_honestly_signed (honestk $k++ ks) msg = true.
   Proof.
@@ -1034,7 +572,7 @@ Section KeyMergeTheorems.
   Qed.
 
   Lemma message_honestly_signed_after_remove_pub_keys :
-    forall {t} (msg : message t) pubk,
+    forall {t} (msg : message t) honestk pubk,
       msg_honestly_signed (honestk $k++ pubk) msg = true
       -> (forall k kp, pubk $? k = Some kp -> kp = false)
       -> msg_honestly_signed honestk msg = true.
@@ -1062,40 +600,8 @@ Section KeyMergeTheorems.
       + rewrite merge_perms_adds_no_new_perms in H; auto.
   Qed.
 
-  (* Lemma message_contains_only_honest_public_keys_after_new_keys : *)
-  (*   forall {t} (msg : message t) msgk, *)
-  (*     msg_contains_only_honest_public_keys honestk msg *)
-  (*     -> msg_contains_only_honest_public_keys (honestk $k++ msgk) msg. *)
-  (* Proof. *)
-  (*   induction 1; econstructor; eauto. *)
-  (*   cases (msgk $? fst kp); eauto. *)
-  (*   erewrite merge_perms_chooses_greatest; eauto; unfold greatest_permission; *)
-  (*     rewrite orb_true_l; trivial. *)
-  (* Qed. *)
-
-  (* Hint Resolve message_honestly_signed_after_new_msg_keys. *)
-
-  (* Lemma message_queue_safe_after_new_message_keys : *)
-  (*   forall {t} (msg : message t) msgs, *)
-  (*     message_queue_safe honestk msgs *)
-  (*     -> message_queue_safe (honestk $k++ findKeys msg) msgs. *)
-  (* Proof. *)
-  (*   unfold message_queue_safe; induction 1; intros; eauto. *)
-  (*   econstructor; eauto. *)
-  (*   destruct x; eauto. *)
-  (* Qed. *)
-
-  (* Lemma message_queue_safe_after_msg_keys : *)
-  (*   forall msgk msgs, *)
-  (*     message_queue_safe honestk msgs *)
-  (*     -> message_queue_safe (honestk $k++ msgk) msgs. *)
-  (* Proof. *)
-  (*   unfold message_queue_safe; induction 1; eauto; intros; econstructor; auto. *)
-  (*   destruct x; eauto. *)
-  (* Qed. *)
-
   Lemma cipher_honestly_signed_after_msg_keys :
-    forall msgk c,
+    forall honestk msgk c,
       cipher_honestly_signed honestk c = true
       -> cipher_honestly_signed (honestk $k++ msgk) c = true.
   Proof.
@@ -1106,14 +612,15 @@ Section KeyMergeTheorems.
   Hint Resolve cipher_honestly_signed_after_msg_keys.
 
   Lemma ciphers_honestly_signed_after_msg_keys :
-    forall msgk cs,
+    forall honestk msgk cs,
       ciphers_honestly_signed honestk cs
       -> ciphers_honestly_signed (honestk $k++ msgk) cs.
   Proof.
     induction 1; econstructor; eauto.
   Qed.
 
-End KeyMergeTheorems.
+End RealWorldLemmas.
+
 
 Lemma safe_messages_have_only_honest_public_keys :
   forall {t} (msg : message t) honestk,
