KeyManagement/Tactics.v
@@ -1,0 +1,36 @@
+From Coq Require Import
+     String
+     Sumbool
+     Eqdep.
+
+Require Import
+        MyPrelude
+        Common
+        Maps.
+
+Set Implicit Arguments.
+
+Ltac context_map_rewrites :=
+  repeat
+    match goal with
+    | [ H : ?m $? ?k = _ |- context[?m $? ?k] ] => rewrite H
+    | [ H : match ?matchee with _ => _ end $? _ = _
+     ,  H1 : ?matchee = _ |- _] => rewrite H1 in H
+    | [ H : match ?matchee with _ => _ end = _
+     ,  H1 : ?matchee = _ |- _] => rewrite H1 in H
+    end.
+
+Ltac invert H :=
+  (MyPrelude.invert H || (inversion H; clear H));
+  repeat match goal with
+         (* | [ x : _ |- _ ] => subst x *)
+         | [ H : existT _ _ _ = existT _ _ _ |- _ ] => apply inj_pair2 in H; try subst
+         end.
+
+Ltac clean_context :=
+  try discriminate;
+  repeat
+    match goal with
+    | [ H : ?X = ?X |- _ ] => clear H
+    | [ H : Some _ = Some _ |- _ ] => invert H
+    end.
